convert LowParse.Pulse back to ghost parsers, serializers (WIP impl_pred_recursive)

src/lowparse/pulse/LowParse.Pulse.Combinators.fst
@@ -13,7 +13,7 @@ inline_for_extraction
 fn validate_ret
   (#t: Type0)
   (x: t)
-: validator #t #parse_ret_kind (tot_parse_ret x)
+: validator #t #parse_ret_kind (parse_ret x)
 = (input: slice byte)
   (poffset: _)
   (#offset: _)
@@ -30,7 +30,7 @@ fn leaf_read_ret
   (#t: Type0)
   (x: t)
   (v_unique: (v' : t) -> Lemma (x == v'))
-: leaf_reader #t #parse_ret_kind #(tot_parse_ret x) (tot_serialize_ret x v_unique)
+: leaf_reader #t #parse_ret_kind #(parse_ret x) (serialize_ret x v_unique)
 = (input: slice byte)
   (#pm: _)
   (#v: _)
@@ -45,29 +45,29 @@ let read_ret
   (#t: Type0)
   (x: t)
   (v_unique: (v' : t) -> Lemma (x == v'))
-: Tot (reader (tot_serialize_ret x v_unique))
+: Tot (reader (serialize_ret x v_unique))
 = reader_of_leaf_reader (leaf_read_ret x v_unique)
 
 inline_for_extraction
-let jump_ret (#t: Type) (x: t) : jumper (tot_parse_ret x) = jump_constant_size (tot_parse_ret x) 0sz 
+let jump_ret (#t: Type) (x: t) : jumper (parse_ret x) = jump_constant_size (parse_ret x) 0sz 
 
 inline_for_extraction
-let validate_empty : validator tot_parse_empty = validate_ret ()
+let validate_empty : validator parse_empty = validate_ret ()
 
 inline_for_extraction
-let leaf_read_empty : leaf_reader tot_serialize_empty = leaf_read_ret () (fun _ -> ())
+let leaf_read_empty : leaf_reader serialize_empty = leaf_read_ret () (fun _ -> ())
 
 inline_for_extraction
-let read_empty : reader tot_serialize_empty = reader_of_leaf_reader leaf_read_empty
+let read_empty : reader serialize_empty = reader_of_leaf_reader leaf_read_empty
 
 inline_for_extraction
-let jump_empty : jumper tot_parse_empty = jump_ret ()
+let jump_empty : jumper parse_empty = jump_ret ()
 
 let parse_serialize_strong_prefix
   (#t: Type)
   (#k: parser_kind)
-  (#p: tot_parser k t)
-  (s: tot_serializer p)
+  (#p: parser k t)
+  (s: serializer p)
   (v: t)
   (suff: bytes)
 : Lemma
@@ -79,33 +79,22 @@ let parse_serialize_strong_prefix
 = let sv = bare_serialize s v in
   parse_strong_prefix #k p sv (sv `Seq.append` suff)
 
-let tot_parse_synth_eq'
-  (#k: parser_kind)
-  (#t1: Type)
-  (#t2: Type)
-  (p1: tot_parser k t1)
-  (f2: (t1 -> Tot t2) {synth_injective f2})
-  (b: bytes)
-: Lemma
-  (ensures (parse (tot_parse_synth p1 f2) b == parse_synth' #k p1 f2 b))
-= parse_synth_eq #k p1 f2 b
-
 inline_for_extraction
 ```pulse
 fn validate_synth
   (#t #t': Type)
-  (#k: parser_kind)
-  (#p: tot_parser k t)
+  (#k: Ghost.erased parser_kind)
+  (#p: parser k t)
   (w: validator p)
-  (f: (t -> t') { synth_injective f })
-: validator #t' #k (tot_parse_synth p f)
+  (f: (t -> GTot t') { synth_injective f })
+: validator #t' #k (parse_synth p f)
 = (input: slice byte)
   (poffset: _)
   (#offset: _)
   (#pm: _)
   (#v: _)
 {
-  tot_parse_synth_eq' p f (Seq.slice v (SZ.v offset) (Seq.length v));
+  parse_synth_eq p f (Seq.slice v (SZ.v offset) (Seq.length v));
   w input poffset #offset #pm #v
 }
 ```
@@ -114,18 +103,18 @@ inline_for_extraction
 ```pulse
 fn jump_synth
   (#t #t': Type0)
-  (#k: parser_kind)
-  (#p: tot_parser k t)
+  (#k: Ghost.erased parser_kind)
+  (#p: parser k t)
   (w: jumper p)
-  (f: (t -> t') { synth_injective f })
-: jumper #t' #k (tot_parse_synth #k #t p f)
+  (f: (t -> GTot t') { synth_injective f })
+: jumper #t' #k (parse_synth #k #t p f)
 =
   (input: _)
   (offset: _)
   (#pm: _)
   (#v: _)
 {    
-  tot_parse_synth_eq' p f (Seq.slice v (SZ.v offset) (Seq.length v));
+  parse_synth_eq p f (Seq.slice v (SZ.v offset) (Seq.length v));
   w input offset #pm #v
 }
 ```
@@ -135,23 +124,23 @@ ghost
 fn pts_to_serialized_synth_intro
   (#t #t': Type0)
   (#k: parser_kind)
-  (#p: tot_parser k t)
-  (s: tot_serializer p)
-  (f: (t -> t') { synth_injective f })
-  (f': (t' -> t) { synth_inverse f f' })
+  (#p: parser k t)
+  (s: serializer p)
+  (f: (t -> GTot t') { synth_injective f })
+  (f': (t' -> GTot t) { synth_inverse f f' })
   (input: slice byte)
   (#pm: perm)
   (#v: t)
   requires pts_to_serialized s input #pm v
-  ensures pts_to_serialized (tot_serialize_synth p f s f' ()) input #pm (f v)
+  ensures pts_to_serialized (serialize_synth p f s f' ()) input #pm (f v)
 {
-  tot_parse_synth_eq p f (bare_serialize s v);
-  parse_serialize #k #t' #(tot_parse_synth p f) (tot_serialize_synth p f s f' ()) (f v);
-  parse_injective #k #t' (tot_parse_synth p f) (bare_serialize s v) (bare_serialize (tot_serialize_synth p f s f' ()) (f v));
+  parse_synth_eq p f (bare_serialize s v);
+  parse_serialize #k #t' #(parse_synth p f) (serialize_synth p f s f' ()) (f v);
+  parse_injective #k #t' (parse_synth p f) (bare_serialize s v) (bare_serialize (serialize_synth p f s f' ()) (f v));
   unfold (pts_to_serialized s input #pm v);
   rewrite (pts_to input #pm (bare_serialize s v))
-    as (pts_to input #pm (bare_serialize (tot_serialize_synth p f s f' ()) (f v)));
-  fold (pts_to_serialized (tot_serialize_synth p f s f' ()) input #pm (f v))
+    as (pts_to input #pm (bare_serialize (serialize_synth p f s f' ()) (f v)));
+  fold (pts_to_serialized (serialize_synth p f s f' ()) input #pm (f v))
 }
 ```
 
@@ -160,21 +149,21 @@ ghost
 fn pts_to_serialized_synth_elim
   (#t #t': Type0)
   (#k: parser_kind)
-  (#p: tot_parser k t)
-  (s: tot_serializer p)
-  (f: (t -> t') { synth_injective f })
-  (f': (t' -> t) { synth_inverse f f' })
+  (#p: parser k t)
+  (s: serializer p)
+  (f: (t -> GTot t') { synth_injective f })
+  (f': (t' -> GTot t) { synth_inverse f f' })
   (input: slice byte)
   (#pm: perm)
   (v: t)
-  requires pts_to_serialized (tot_serialize_synth p f s f' ()) input #pm (f v)
+  requires pts_to_serialized (serialize_synth p f s f' ()) input #pm (f v)
   ensures pts_to_serialized s input #pm v
 {
-  tot_parse_synth_eq p f (bare_serialize s v);
-  parse_serialize #k #t' #(tot_parse_synth p f) (tot_serialize_synth p f s f' ()) (f v);
-  parse_injective #k #t' (tot_parse_synth p f) (bare_serialize s v) (bare_serialize (tot_serialize_synth p f s f' ()) (f v));
-  unfold (pts_to_serialized (tot_serialize_synth p f s f' ()) input #pm (f v));
-  rewrite (pts_to input #pm (bare_serialize (tot_serialize_synth p f s f' ()) (f v)))
+  parse_synth_eq p f (bare_serialize s v);
+  parse_serialize #k #t' #(parse_synth p f) (serialize_synth p f s f' ()) (f v);
+  parse_injective #k #t' (parse_synth p f) (bare_serialize s v) (bare_serialize (serialize_synth p f s f' ()) (f v));
+  unfold (pts_to_serialized (serialize_synth p f s f' ()) input #pm (f v));
+  rewrite (pts_to input #pm (bare_serialize (serialize_synth p f s f' ()) (f v)))
     as (pts_to input #pm (bare_serialize s v));
   fold (pts_to_serialized s input #pm v)
 }
@@ -185,21 +174,21 @@ ghost
 fn pts_to_serialized_synth_trade
   (#t #t': Type0)
   (#k: parser_kind)
-  (#p: tot_parser k t)
-  (s: tot_serializer p)
-  (f: (t -> t') { synth_injective f })
-  (f': (t' -> t) { synth_inverse f f' })
+  (#p: parser k t)
+  (s: serializer p)
+  (f: (t -> GTot t') { synth_injective f })
+  (f': (t' -> GTot t) { synth_inverse f f' })
   (input: slice byte)
   (#pm: perm)
   (#v: t)
   requires pts_to_serialized s input #pm v
-  ensures pts_to_serialized (tot_serialize_synth p f s f' ()) input #pm (f v) ** trade (pts_to_serialized (tot_serialize_synth p f s f' ()) input #pm (f v)) (pts_to_serialized s input #pm v)
+  ensures pts_to_serialized (serialize_synth p f s f' ()) input #pm (f v) ** trade (pts_to_serialized (serialize_synth p f s f' ()) input #pm (f v)) (pts_to_serialized s input #pm v)
 {
   pts_to_serialized_synth_intro s f f' input;
   ghost
   fn aux
     (_: unit)
-    requires emp ** pts_to_serialized (tot_serialize_synth p f s f' ()) input #pm (f v)
+    requires emp ** pts_to_serialized (serialize_synth p f s f' ()) input #pm (f v)
     ensures pts_to_serialized s input #pm v
   {
     pts_to_serialized_synth_elim s f f' input v 
@@ -213,18 +202,18 @@ ghost
 fn pts_to_serialized_synth_l2r
   (#t #t': Type0)
   (#k: parser_kind)
-  (#p: tot_parser k t)
-  (s: tot_serializer p)
-  (f: (t -> t') { synth_injective f })
-  (f': (t' -> t) { synth_inverse f f' })
+  (#p: parser k t)
+  (s: serializer p)
+  (f: (t -> GTot t') { synth_injective f })
+  (f': (t' -> GTot t) { synth_inverse f f' })
   (input: slice byte)
   (#pm: perm)
   (#v: t')
-  requires pts_to_serialized (tot_serialize_synth p f s f' ()) input #pm v
+  requires pts_to_serialized (serialize_synth p f s f' ()) input #pm v
   ensures pts_to_serialized s input #pm (f' v)
 {
-  tot_serialize_synth_eq p f s f' () v;
-  unfold (pts_to_serialized (tot_serialize_synth p f s f' ()) input #pm v);
+  serialize_synth_eq p f s f' () v;
+  unfold (pts_to_serialized (serialize_synth p f s f' ()) input #pm v);
   fold (pts_to_serialized s input #pm (f' v))
 }
 ```
@@ -234,19 +223,19 @@ ghost
 fn pts_to_serialized_synth_r2l
   (#t #t': Type0)
   (#k: parser_kind)
-  (#p: tot_parser k t)
-  (s: tot_serializer p)
-  (f: (t -> t') { synth_injective f })
-  (f': (t' -> t) { synth_inverse f f' })
+  (#p: parser k t)
+  (s: serializer p)
+  (f: (t -> GTot t') { synth_injective f })
+  (f': (t' -> GTot t) { synth_inverse f f' })
   (input: slice byte)
   (#pm: perm)
   (v: t')
   requires pts_to_serialized s input #pm (f' v)
-  ensures pts_to_serialized (tot_serialize_synth p f s f' ()) input #pm v
+  ensures pts_to_serialized (serialize_synth p f s f' ()) input #pm v
 {
-  tot_serialize_synth_eq p f s f' () v;
+  serialize_synth_eq p f s f' () v;
   unfold (pts_to_serialized s input #pm (f' v));
-  fold (pts_to_serialized (tot_serialize_synth p f s f' ()) input #pm v)
+  fold (pts_to_serialized (serialize_synth p f s f' ()) input #pm v)
 }
 ```
 
@@ -255,22 +244,22 @@ ghost
 fn pts_to_serialized_synth_l2r_trade
   (#t #t': Type0)
   (#k: parser_kind)
-  (#p: tot_parser k t)
-  (s: tot_serializer p)
-  (f: (t -> t') { synth_injective f })
-  (f': (t' -> t) { synth_inverse f f' })
+  (#p: parser k t)
+  (s: serializer p)
+  (f: (t -> GTot t') { synth_injective f })
+  (f': (t' -> GTot t) { synth_inverse f f' })
   (input: slice byte)
   (#pm: perm)
   (#v: t')
-  requires pts_to_serialized (tot_serialize_synth p f s f' ()) input #pm v
-  ensures pts_to_serialized s input #pm (f' v) ** trade (pts_to_serialized s input #pm (f' v)) (pts_to_serialized (tot_serialize_synth p f s f' ()) input #pm v)
+  requires pts_to_serialized (serialize_synth p f s f' ()) input #pm v
+  ensures pts_to_serialized s input #pm (f' v) ** trade (pts_to_serialized s input #pm (f' v)) (pts_to_serialized (serialize_synth p f s f' ()) input #pm v)
 {
   pts_to_serialized_synth_l2r s f f' input;
   ghost
   fn aux
     (_: unit)
     requires emp ** pts_to_serialized s input #pm (f' v)
-    ensures pts_to_serialized (tot_serialize_synth p f s f' ()) input #pm v
+    ensures pts_to_serialized (serialize_synth p f s f' ()) input #pm v
   {
     pts_to_serialized_synth_r2l s f f' input v
   };
@@ -283,22 +272,22 @@ ghost
 fn pts_to_serialized_synth_l2r_trade'
   (#t #t': Type0)
   (#k_: parser_kind)
-  (#p_: tot_parser k_ t')
-  (#s_: tot_serializer p_)
+  (#p_: parser k_ t')
+  (#s_: serializer p_)
   (#k: parser_kind)
-  (#p: tot_parser k t)
-  (s: tot_serializer p)
-  (f: (t -> t') { synth_injective f })
-  (f': (t' -> t) { synth_inverse f f' })
+  (#p: parser k t)
+  (s: serializer p)
+  (f: (t -> GTot t') { synth_injective f })
+  (f': (t' -> GTot t) { synth_inverse f f' })
   (input: slice byte)
   (#pm: perm)
   (#v: t')
-  requires pts_to_serialized s_ input #pm v ** pure (forall x . parse p_ x == parse (tot_parse_synth p f) x)
+  requires pts_to_serialized s_ input #pm v ** pure (forall x . parse p_ x == parse (parse_synth p f) x)
   ensures pts_to_serialized s input #pm (f' v) ** trade (pts_to_serialized s input #pm (f' v)) (pts_to_serialized s_ input #pm v)
 {
   pts_to_serialized_ext_trade
     s_
-    (tot_serialize_synth p f s f' ())
+    (serialize_synth p f s f' ())
     input;
   pts_to_serialized_synth_l2r_trade
     s f f' input;
@@ -315,7 +304,7 @@ let read_synth_cont_t
 inline_for_extraction
 let read_synth_cont
   (#t1 #t2: Type0)
-  (f2: (t1 -> Tot t2))
+  (f2: (t1 -> GTot t2))
   (f2': ((x: t1) -> read_synth_cont_t (f2 x)))
   (x1: Ghost.erased t1)
   (t': Type0)
@@ -327,10 +316,10 @@ let read_synth_cont
 inline_for_extraction
 ```pulse
 fn read_synth
-  (#k1: parser_kind) (#t1: Type0) (#p1: parser k1 t1) (#s1: serializer p1) (r: reader s1)
-  (#t2: Type0) (f2: (t1 -> Tot t2) { synth_injective f2 }) (f1: (t2 -> Tot t1) { synth_inverse f2 f1 })
+  (#k1: Ghost.erased parser_kind) (#t1: Type0) (#p1: parser k1 t1) (#s1: serializer p1) (r: reader s1)
+  (#t2: Type0) (f2: (t1 -> GTot t2) { synth_injective f2 }) (f1: (t2 -> GTot t1) { synth_inverse f2 f1 })
   (f2': ((x: t1) -> read_synth_cont_t (f2 x)))
-: reader #t2 #k1 #(tot_parse_synth p1 f2) (tot_serialize_synth p1 f2 s1 f1 ())
+: reader #t2 #k1 #(parse_synth p1 f2) (serialize_synth p1 f2 s1 f1 ())
 = (input: slice byte)
   (#pm: _)
   (#v: _)
@@ -353,23 +342,23 @@ let read_synth_cont_init
 
 inline_for_extraction
 let read_synth'
-  (#k1: parser_kind) (#t1: Type0) (#p1: parser k1 t1) (#s1: serializer p1) (r: reader s1)
-  (#t2: Type0) (f2: (t1 -> Tot t2) { synth_injective f2 }) (f1: (t2 -> Tot t1) { synth_inverse f2 f1 })
-: reader #t2 #k1 #(tot_parse_synth p1 f2) (tot_serialize_synth p1 f2 s1 f1 ())
+  (#k1: Ghost.erased parser_kind) (#t1: Type0) (#p1: parser k1 t1) (#s1: serializer p1) (r: reader s1)
+  (#t2: Type0) (f2: (t1 -> Tot t2) { synth_injective f2 }) (f1: (t2 -> GTot t1) { synth_inverse f2 f1 })
+: reader #t2 #k1 #(parse_synth p1 f2) (serialize_synth p1 f2 s1 f1 ())
 = read_synth r f2 f1 (fun x -> read_synth_cont_init (f2 x))
 
 inline_for_extraction
 ```pulse
 fn validate_filter
   (#t: Type0)
-  (#k: parser_kind)
-  (#p: tot_parser k t)
+  (#k: Ghost.erased parser_kind)
+  (#p: parser k t)
   (w: validator p)
   (#s: serializer p)
   (r: leaf_reader s)
-  (f: (t -> bool))
+  (f: (t -> GTot bool))
   (f': (x: t) -> (y: bool { y == f x }))
-: validator #_ #(parse_filter_kind k) (tot_parse_filter p f)
+: validator #_ #(parse_filter_kind k) (parse_filter p f)
 =
   (input: slice byte)
   (poffset: _)
@@ -377,7 +366,7 @@ fn validate_filter
   (#pm: perm)
   (#v: Ghost.erased bytes)
 {
-  tot_parse_filter_eq p f (Seq.slice v (SZ.v offset) (Seq.length v));
+  parse_filter_eq p f (Seq.slice v (SZ.v offset) (Seq.length v));
   let offset = !poffset;
   let is_valid = w input poffset;
   if is_valid {
@@ -401,31 +390,31 @@ let validate_filter'_test
 inline_for_extraction
 let validate_filter'
   (#t: Type0)
-  (#k: parser_kind)
-  (#p: tot_parser k t)
+  (#k: Ghost.erased parser_kind)
+  (#p: parser k t)
   (w: validator p)
   (#s: serializer p)
   (r: leaf_reader s)
   (f: (t -> bool))
-: validator #_ #(parse_filter_kind k) (tot_parse_filter p f)
+: validator #_ #(parse_filter_kind k) (parse_filter p f)
 = validate_filter w r f (validate_filter'_test f)
 
 inline_for_extraction
 ```pulse
 fn jump_filter
   (#t: Type0)
-  (#k: parser_kind)
-  (#p: tot_parser k t)
+  (#k: Ghost.erased parser_kind)
+  (#p: parser k t)
   (w: jumper p)
-  (f: (t -> bool))
-: jumper #_ #(parse_filter_kind k) (tot_parse_filter p f)
+  (f: (t -> GTot bool))
+: jumper #_ #(parse_filter_kind k) (parse_filter p f)
 =
   (input: slice byte)
   (offset: SZ.t)
   (#pm: perm)
   (#v: Ghost.erased bytes)
 {
-  Classical.forall_intro (tot_parse_filter_eq p f);
+  Classical.forall_intro (parse_filter_eq p f);
   w input offset #pm #v
 }
 ```
@@ -444,17 +433,17 @@ ghost
 fn pts_to_serialized_filter_intro
   (#t: Type0)
   (#k: parser_kind)
-  (#p: tot_parser k t)
+  (#p: parser k t)
   (s: serializer p)
-  (f: (t -> bool))
+  (f: (t -> GTot bool))
   (input: slice byte)
   (#pm: perm)
   (#v: t)
   requires (pts_to_serialized s input #pm v ** pure (f v == true))
-  ensures exists* (v': parse_filter_refine f) . pts_to_serialized (tot_serialize_filter s f) input #pm v' ** pure ((v' <: t) == v)
+  ensures exists* (v': parse_filter_refine f) . pts_to_serialized (serialize_filter s f) input #pm v' ** pure ((v' <: t) == v)
 {
   unfold (pts_to_serialized s input #pm v);
-  fold (pts_to_serialized (tot_serialize_filter s f) input #pm v);
+  fold (pts_to_serialized (serialize_filter s f) input #pm v);
 }
 ```
 
@@ -463,16 +452,16 @@ ghost
 fn pts_to_serialized_filter_elim
   (#t: Type0)
   (#k: parser_kind)
-  (#p: tot_parser k t)
+  (#p: parser k t)
   (s: serializer p)
-  (f: (t -> bool))
+  (f: (t -> GTot bool))
   (input: slice byte)
   (#pm: perm)
   (#v: parse_filter_refine f)
-  requires (pts_to_serialized (tot_serialize_filter s f) input #pm v)
+  requires (pts_to_serialized (serialize_filter s f) input #pm v)
   ensures pts_to_serialized s input #pm v
 {
-  unfold (pts_to_serialized (tot_serialize_filter s f) input #pm v);
+  unfold (pts_to_serialized (serialize_filter s f) input #pm v);
   fold (pts_to_serialized s input #pm v);
 }
 ```
@@ -480,7 +469,7 @@ fn pts_to_serialized_filter_elim
 inline_for_extraction
 let read_filter_cont
   (#t: Type0)
-  (f: t -> bool)
+  (f: t -> GTot bool)
   (v: Ghost.erased (parse_filter_refine f))
   (t': Type0)
   (g: (x: parse_filter_refine f { x == Ghost.reveal v }) -> t')
@@ -491,8 +480,8 @@ let read_filter_cont
 inline_for_extraction
 ```pulse
 fn read_filter
-  (#k1: parser_kind) (#t1: Type0) (#p1: parser k1 t1) (#s1: serializer p1) (r: reader s1) (f: (t1 -> bool))
-: reader #(parse_filter_refine f) #(parse_filter_kind k1) #(tot_parse_filter p1 f) (tot_serialize_filter s1 f)
+  (#k1: Ghost.erased parser_kind) (#t1: Type0) (#p1: parser k1 t1) (#s1: serializer p1) (r: reader s1) (f: (t1 -> GTot bool))
+: reader #(parse_filter_refine f) #(parse_filter_kind k1) #(parse_filter p1 f) (serialize_filter s1 f)
 = (input: slice byte)
   (#pm: _)
   (#v: _)
@@ -523,25 +512,26 @@ let dtuple2_of_pair
 let nondep_then_eq_dtuple2
   (#t1 #t2: Type)
   (#k1 #k2: parser_kind)
-  (p1: tot_parser k1 t1)
-  (p2: tot_parser k2 t2)
+  (p1: parser k1 t1)
+  (p2: parser k2 t2)
   (input: bytes)
 : Lemma
-  (parse (tot_nondep_then p1 p2) input == parse (tot_parse_synth (tot_parse_dtuple2 p1 (fun _ -> p2)) pair_of_dtuple2) input)
-= tot_parse_synth_eq (tot_parse_dtuple2 p1 (fun _ -> p2)) pair_of_dtuple2 input;
+  (parse (nondep_then p1 p2) input == parse (parse_synth (parse_dtuple2 p1 (fun _ -> p2)) pair_of_dtuple2) input)
+= parse_synth_eq (parse_dtuple2 p1 (fun _ -> p2)) pair_of_dtuple2 input;
+  parse_dtuple2_eq p1 (fun _ -> p2) input;
   nondep_then_eq #k1 #t1 p1 #k2 #t2 p2 input
 
 inline_for_extraction
 ```pulse
 fn validate_nondep_then
   (#t1 #t2: Type0)
-  (#k1: parser_kind)
+  (#k1: Ghost.erased parser_kind)
   (#p1: parser k1 t1)
   (v1: validator p1)
-  (#k2: parser_kind)
+  (#k2: Ghost.erased parser_kind)
   (#p2: parser k2 t2)
   (v2: validator p2)
-: validator #(t1 & t2) #(and_then_kind k1 k2) (tot_nondep_then #k1 #t1 p1 #k2 #t2 p2)
+: validator #(t1 & t2) #(and_then_kind k1 k2) (nondep_then #k1 #t1 p1 #k2 #t2 p2)
 = 
   (input: slice byte)
   (poffset: _)
@@ -564,15 +554,15 @@ inline_for_extraction
 fn validate_dtuple2
   (#t1: Type0)
   (#t2: t1 -> Type0)
-  (#k1: parser_kind)
+  (#k1: Ghost.erased parser_kind)
   (#p1: parser k1 t1)
   (v1: validator p1)
   (#s1: serializer p1)
   (r1: leaf_reader s1)
-  (#k2: parser_kind)
+  (#k2: Ghost.erased parser_kind)
   (#p2: ((x: t1) -> parser k2 (t2 x)))
   (v2: ((x: t1) -> validator (p2 x)))
-: validator #(dtuple2 t1 t2) #(and_then_kind k1 k2) (tot_parse_dtuple2 #k1 #t1 p1 #k2 #t2 p2)
+: validator #(dtuple2 t1 t2) #(and_then_kind k1 k2) (parse_dtuple2 #k1 #t1 p1 #k2 #t2 p2)
 =
   (input: slice byte)
   (poffset: _)
@@ -580,6 +570,7 @@ fn validate_dtuple2
   (#pm: perm)
   (#v: Ghost.erased bytes)
 {
+  parse_dtuple2_eq p1 p2 (Seq.slice v (SZ.v offset) (Seq.length v));
   let offset = !poffset;
   let is_valid1 = v1 input poffset;
   if is_valid1 {
@@ -596,13 +587,13 @@ inline_for_extraction
 ```pulse
 fn jump_nondep_then
   (#t1 #t2: Type0)
-  (#k1: parser_kind)
+  (#k1: Ghost.erased parser_kind)
   (#p1: parser k1 t1)
   (v1: jumper p1)
-  (#k2: parser_kind)
+  (#k2: Ghost.erased parser_kind)
   (#p2: parser k2 t2)
   (v2: jumper p2)
-: jumper #(t1 & t2) #(and_then_kind k1 k2) (tot_nondep_then #k1 #t1 p1 #k2 #t2 p2)
+: jumper #(t1 & t2) #(and_then_kind k1 k2) (nondep_then #k1 #t1 p1 #k2 #t2 p2)
 = 
   (input: slice byte)
   (offset: SZ.t)
@@ -621,21 +612,22 @@ inline_for_extraction
 fn jump_dtuple2
   (#t1: Type0)
   (#t2: t1 -> Type0)
-  (#k1: parser_kind)
+  (#k1: Ghost.erased parser_kind)
   (#p1: parser k1 t1)
   (v1: jumper p1)
   (#s1: serializer p1)
   (r1: leaf_reader s1)
-  (#k2: parser_kind)
+  (#k2: Ghost.erased parser_kind)
   (#p2: (x: t1) -> parser k2 (t2 x))
   (v2: (x: t1) -> jumper (p2 x))
-: jumper #(dtuple2 t1 t2) #(and_then_kind k1 k2) (tot_parse_dtuple2 #k1 #t1 p1 #k2 #t2 p2)
+: jumper #(dtuple2 t1 t2) #(and_then_kind k1 k2) (parse_dtuple2 #k1 #t1 p1 #k2 #t2 p2)
 = 
   (input: slice byte)
   (offset: SZ.t)
   (#pm: perm)
   (#v: Ghost.erased bytes)
 {
+  parse_dtuple2_eq p1 p2 (Seq.slice v (SZ.v offset) (Seq.length v));
   pts_to_len input;
   let off1 = v1 input offset;
   let x = read_from_validator_success r1 input offset off1;
@@ -661,7 +653,7 @@ let split_dtuple2_post'
   pts_to_serialized (s2 (dfst v)) right #pm (dsnd v) **
   trade (pts_to_serialized s1 left #pm (dfst v) **
   pts_to_serialized (s2 (dfst v)) right #pm (dsnd v))
-    (pts_to_serialized (tot_serialize_dtuple2 s1 s2) input #pm v)
+    (pts_to_serialized (serialize_dtuple2 s1 s2) input #pm v)
 
 let split_dtuple2_post
   (#t1: Type0)
@@ -685,22 +677,23 @@ inline_for_extraction
 fn split_dtuple2
   (#t1: Type0)
   (#t2: t1 -> Type0)
-  (#k1: parser_kind)
+  (#k1: Ghost.erased parser_kind)
   (#p1: parser k1 t1)
   (s1: serializer p1 { k1.parser_kind_subkind == Some ParserStrong })
   (j1: jumper p1)
-  (#k2: parser_kind)
+  (#k2: Ghost.erased parser_kind)
   (#p2: ((x: t1) -> parser k2 (t2 x)))
   (s2: (x: t1) -> serializer (p2 x))
   (input: slice byte)
   (#pm: perm)
   (#v: Ghost.erased (dtuple2 t1 t2))
-  requires pts_to_serialized (tot_serialize_dtuple2 s1 s2) input #pm v
+  requires pts_to_serialized (serialize_dtuple2 s1 s2) input #pm v
   returns res: slice_pair byte
   ensures split_dtuple2_post s1 s2 input pm v res
 {
+  serialize_dtuple2_eq s1 s2 v;
   Trade.rewrite_with_trade
-    (pts_to_serialized (tot_serialize_dtuple2 s1 s2) input #pm v)
+    (pts_to_serialized (serialize_dtuple2 s1 s2) input #pm v)
     (pts_to input #pm (bare_serialize s1 (dfst v) `Seq.append` bare_serialize (s2 (dfst v)) (dsnd v)));
   parse_serialize_strong_prefix s1 (dfst v) (bare_serialize (s2 (dfst v)) (dsnd v));
   let i = j1 input 0sz;
@@ -727,20 +720,20 @@ inline_for_extraction
 fn dtuple2_dfst
   (#t1: Type0)
   (#t2: t1 -> Type0)
-  (#k1: parser_kind)
+  (#k1: Ghost.erased parser_kind)
   (#p1: parser k1 t1)
   (s1: serializer p1 { k1.parser_kind_subkind == Some ParserStrong })
   (j1: jumper p1)
-  (#k2: parser_kind)
+  (#k2: Ghost.erased parser_kind)
   (#p2: ((x: t1) -> parser k2 (t2 x)))
   (s2: (x: t1) -> serializer (p2 x))
   (input: slice byte)
   (#pm: perm)
   (#v: Ghost.erased (dtuple2 t1 t2))
-  requires pts_to_serialized (tot_serialize_dtuple2 s1 s2) input #pm v
+  requires pts_to_serialized (serialize_dtuple2 s1 s2) input #pm v
   returns res: slice byte
   ensures pts_to_serialized s1 res #pm (dfst v) **
-    trade (pts_to_serialized s1 res #pm (dfst v)) (pts_to_serialized (tot_serialize_dtuple2 s1 s2) input #pm v)
+    trade (pts_to_serialized s1 res #pm (dfst v)) (pts_to_serialized (serialize_dtuple2 s1 s2) input #pm v)
 {
   let spl = split_dtuple2 s1 j1 s2 input;
   match spl { SlicePair input1 input2 -> {
@@ -757,20 +750,20 @@ inline_for_extraction
 fn dtuple2_dsnd
   (#t1: Type0)
   (#t2: t1 -> Type0)
-  (#k1: parser_kind)
+  (#k1: Ghost.erased parser_kind)
   (#p1: parser k1 t1)
   (s1: serializer p1 { k1.parser_kind_subkind == Some ParserStrong })
   (j1: jumper p1)
-  (#k2: parser_kind)
+  (#k2: Ghost.erased parser_kind)
   (#p2: ((x: t1) -> parser k2 (t2 x)))
   (s2: (x: t1) -> serializer (p2 x))
   (input: slice byte)
   (#pm: perm)
   (#v: Ghost.erased (dtuple2 t1 t2))
-  requires pts_to_serialized (tot_serialize_dtuple2 s1 s2) input #pm v
+  requires pts_to_serialized (serialize_dtuple2 s1 s2) input #pm v
   returns res: slice byte
   ensures pts_to_serialized (s2 (dfst v)) res #pm (dsnd v) **
-    trade (pts_to_serialized (s2 (dfst v)) res #pm (dsnd v)) (pts_to_serialized (tot_serialize_dtuple2 s1 s2) input #pm v)
+    trade (pts_to_serialized (s2 (dfst v)) res #pm (dsnd v)) (pts_to_serialized (serialize_dtuple2 s1 s2) input #pm v)
 {
   let spl = split_dtuple2 s1 j1 s2 input;
   match spl { SlicePair input1 input2 -> {
@@ -799,7 +792,7 @@ let split_nondep_then_post'
   pts_to_serialized s2 right #pm (snd v) **
   trade (pts_to_serialized s1 left #pm (fst v) **
   pts_to_serialized s2 right #pm (snd v))
-    (pts_to_serialized (tot_serialize_nondep_then s1 s2) input #pm v)
+    (pts_to_serialized (serialize_nondep_then s1 s2) input #pm v)
 
 let split_nondep_then_post
   (#t1 #t2: Type0)
@@ -821,37 +814,37 @@ inline_for_extraction
 ```pulse
 fn split_nondep_then
   (#t1 #t2: Type0)
-  (#k1: parser_kind)
+  (#k1: Ghost.erased parser_kind)
   (#p1: parser k1 t1)
   (s1: serializer p1 { k1.parser_kind_subkind == Some ParserStrong })
   (j1: jumper p1)
-  (#k2: parser_kind)
+  (#k2: Ghost.erased parser_kind)
   (#p2: parser k2 t2)
   (s2: serializer p2)
   (input: slice byte)
   (#pm: perm)
   (#v: Ghost.erased (t1 & t2))
-  requires pts_to_serialized (tot_serialize_nondep_then s1 s2) input #pm v
+  requires pts_to_serialized (serialize_nondep_then s1 s2) input #pm v
   returns res: slice_pair byte
   ensures split_nondep_then_post s1 s2 input pm v res
 {
   Classical.forall_intro (nondep_then_eq_dtuple2 p1 p2);
   pts_to_serialized_ext_trade
-    (tot_serialize_nondep_then s1 s2)
-    (tot_serialize_synth
-      (tot_parse_dtuple2 p1 (fun _ -> p2))
+    (serialize_nondep_then s1 s2)
+    (serialize_synth
+      (parse_dtuple2 p1 (fun _ -> p2))
       pair_of_dtuple2
-      (tot_serialize_dtuple2 s1 (fun _ -> s2))
+      (serialize_dtuple2 s1 (fun _ -> s2))
       dtuple2_of_pair
       ()
     )
     input;
   pts_to_serialized_synth_l2r_trade
-    (tot_serialize_dtuple2 s1 (fun _ -> s2))
+    (serialize_dtuple2 s1 (fun _ -> s2))
     pair_of_dtuple2
     dtuple2_of_pair
     input;
-  Trade.trans (pts_to_serialized (tot_serialize_dtuple2 s1 (fun _ -> s2)) _ #pm _) _ _;
+  Trade.trans (pts_to_serialized (serialize_dtuple2 s1 (fun _ -> s2)) _ #pm _) _ _;
   let res = split_dtuple2 s1 j1 (fun _ -> s2) input;
   match res { SlicePair input1 input2 -> {
     unfold (split_dtuple2_post s1 (fun _ -> s2) input pm (dtuple2_of_pair v) res);
@@ -868,20 +861,20 @@ inline_for_extraction
 ```pulse
 fn nondep_then_fst
   (#t1 #t2: Type0)
-  (#k1: parser_kind)
+  (#k1: Ghost.erased parser_kind)
   (#p1: parser k1 t1)
   (s1: serializer p1 { k1.parser_kind_subkind == Some ParserStrong })
   (j1: jumper p1)
-  (#k2: parser_kind)
+  (#k2: Ghost.erased parser_kind)
   (#p2: parser k2 t2)
   (s2: serializer p2)
   (input: slice byte)
   (#pm: perm)
   (#v: Ghost.erased (t1 & t2))
-  requires pts_to_serialized (tot_serialize_nondep_then s1 s2) input #pm v
+  requires pts_to_serialized (serialize_nondep_then s1 s2) input #pm v
   returns res: slice byte
   ensures pts_to_serialized s1 res #pm (fst v) **
-    trade (pts_to_serialized s1 res #pm (fst v)) (pts_to_serialized (tot_serialize_nondep_then s1 s2) input #pm v)
+    trade (pts_to_serialized s1 res #pm (fst v)) (pts_to_serialized (serialize_nondep_then s1 s2) input #pm v)
 {
   let spl = split_nondep_then s1 j1 s2 input;
   match spl { SlicePair input1 input2 -> {
@@ -897,20 +890,20 @@ inline_for_extraction
 ```pulse
 fn nondep_then_snd
   (#t1 #t2: Type0)
-  (#k1: parser_kind)
+  (#k1: Ghost.erased parser_kind)
   (#p1: parser k1 t1)
   (s1: serializer p1 { k1.parser_kind_subkind == Some ParserStrong })
   (j1: jumper p1)
-  (#k2: parser_kind)
+  (#k2: Ghost.erased parser_kind)
   (#p2: parser k2 t2)
   (s2: serializer p2)
   (input: slice byte)
   (#pm: perm)
   (#v: Ghost.erased (t1 & t2))
-  requires pts_to_serialized (tot_serialize_nondep_then s1 s2) input #pm v
+  requires pts_to_serialized (serialize_nondep_then s1 s2) input #pm v
   returns res: slice byte
   ensures pts_to_serialized s2 res #pm (snd v) **
-    trade (pts_to_serialized s2 res #pm (snd v)) (pts_to_serialized (tot_serialize_nondep_then s1 s2) input #pm v)
+    trade (pts_to_serialized s2 res #pm (snd v)) (pts_to_serialized (serialize_nondep_then s1 s2) input #pm v)
 {
   let spl = split_nondep_then s1 j1 s2 input;
   match spl { SlicePair input1 input2 -> {
@@ -927,16 +920,16 @@ inline_for_extraction
 fn read_dtuple2
   (#t1: Type0)
   (#t2: t1 -> Type0)
-  (#k1: parser_kind)
+  (#k1: Ghost.erased parser_kind)
   (#p1: parser k1 t1)
   (j1: jumper p1 { k1.parser_kind_subkind == Some ParserStrong })
   (#s1: serializer p1)
   (r1: reader s1)
-  (#k2: parser_kind)
+  (#k2: Ghost.erased parser_kind)
   (#p2: (x: t1) -> parser k2 (t2 x))
   (#s2: (x: t1) -> serializer (p2 x))
   (r2: (x: t1) -> reader (s2 x))
-: reader #(dtuple2 t1 t2) #(and_then_kind k1 k2) #(tot_parse_dtuple2 p1 p2) (tot_serialize_dtuple2 s1 s2)
+: reader #(dtuple2 t1 t2) #(and_then_kind k1 k2) #(parse_dtuple2 p1 p2) (serialize_dtuple2 s1 s2)
 =   
   (input: slice byte)
   (#pm: perm)
