src/lowparse/pulse/LowParse.Pulse.VCList.fst
@@ -13,11 +13,11 @@ inline_for_extraction
 ```pulse
 fn jump_nlist
    (#t: Type0)
-   (#k: parser_kind)
+   (#k: Ghost.erased parser_kind)
    (#p: parser k t)
    (j: jumper p)
    (n0: SZ.t)
-: jumper #(nlist (SZ.v n0) t) #(parse_nlist_kind (SZ.v n0) k) (tot_parse_nlist (SZ.v n0) p)
+: jumper #(nlist (SZ.v n0) t) #(parse_nlist_kind (SZ.v n0) k) (parse_nlist (SZ.v n0) p)
 =
   (input: slice byte)
   (offset0: SZ.t)
@@ -32,15 +32,15 @@ fn jump_nlist
   ) invariant b . exists* n offset . (
     pts_to input #pm v ** R.pts_to pn n ** R.pts_to poffset offset ** pure (
     SZ.v offset <= Seq.length v /\ (
-    let pr0 = parse_consume (tot_parse_nlist (SZ.v n0) p) (Seq.slice v (SZ.v offset0) (Seq.length v)) in
-    let pr = parse_consume (tot_parse_nlist (SZ.v n) p) (Seq.slice v (SZ.v offset) (Seq.length v)) in
+    let pr0 = parse_consume (parse_nlist (SZ.v n0) p) (Seq.slice v (SZ.v offset0) (Seq.length v)) in
+    let pr = parse_consume (parse_nlist (SZ.v n) p) (Seq.slice v (SZ.v offset) (Seq.length v)) in
     Some? pr0 /\ Some? pr /\
     SZ.v offset0 + Some?.v pr0 == SZ.v offset + Some?.v pr /\
     b == (SZ.v n > 0)
   ))) {
     let n = !pn;
     let offset = !poffset;
-    tot_parse_nlist_eq (SZ.v n) p (Seq.slice v (SZ.v offset) (Seq.length v));
+    parse_nlist_eq (SZ.v n) p (Seq.slice v (SZ.v offset) (Seq.length v));
     let offset' = j input offset;
     pn := (SZ.sub n 1sz);
     poffset := offset';
@@ -61,10 +61,10 @@ fn nlist_cons_as_nondep_then
   (#pm: perm)
   (#v: nlist n t)
 requires
-  pts_to_serialized (tot_serialize_nlist n s) input #pm v
+  pts_to_serialized (serialize_nlist n s) input #pm v
 ensures exists* v' .
-  pts_to_serialized (tot_serialize_nondep_then s (tot_serialize_nlist (n - 1) s)) input #pm v' **
-  trade (pts_to_serialized (tot_serialize_nondep_then s (tot_serialize_nlist (n - 1) s)) input #pm v') (pts_to_serialized (tot_serialize_nlist n s) input #pm v) **
+  pts_to_serialized (serialize_nondep_then s (serialize_nlist (n - 1) s)) input #pm v' **
+  trade (pts_to_serialized (serialize_nondep_then s (serialize_nlist (n - 1) s)) input #pm v') (pts_to_serialized (serialize_nlist n s) input #pm v) **
   pure (
     v == (fst v' :: snd v')
   )
@@ -72,14 +72,14 @@ ensures exists* v' .
   synth_inverse_1 t (n - 1);
   synth_inverse_2 t (n - 1);
   Trade.rewrite_with_trade
-    (pts_to_serialized (tot_serialize_nlist n s) input #pm v)
-    (pts_to_serialized (tot_serialize_synth _ (synth_nlist (n - 1)) (tot_serialize_nondep_then s (tot_serialize_nlist' (n - 1) s)) (synth_nlist_recip (n - 1)) ()) input #pm v);
+    (pts_to_serialized (serialize_nlist n s) input #pm v)
+    (pts_to_serialized (serialize_synth _ (synth_nlist (n - 1)) (serialize_nondep_then s (serialize_nlist' (n - 1) s)) (synth_nlist_recip (n - 1)) ()) input #pm v);
   pts_to_serialized_synth_l2r_trade
-    (tot_serialize_nondep_then s (tot_serialize_nlist' (n - 1) s))
+    (serialize_nondep_then s (serialize_nlist' (n - 1) s))
     (synth_nlist (n - 1))
     (synth_nlist_recip (n - 1))
     input;
-  Trade.trans (pts_to_serialized (tot_serialize_nondep_then s (tot_serialize_nlist (n - 1) s)) input #pm _) _ _
+  Trade.trans (pts_to_serialized (serialize_nondep_then s (serialize_nlist (n - 1) s)) input #pm _) _ _
 }
 ```
 
@@ -87,27 +87,27 @@ inline_for_extraction
 ```pulse
 fn nlist_hd
   (#t: Type0)
-  (#k: parser_kind)
+  (#k: Ghost.erased parser_kind)
   (#p: parser k t)
   (s: serializer p { k.parser_kind_subkind == Some ParserStrong })
   (j: jumper p)
-  (n: pos)
+  (n: Ghost.erased pos)
   (input: slice byte)
   (#pm: perm)
   (#v: Ghost.erased (nlist n t))
 requires
-  pts_to_serialized (tot_serialize_nlist n s) input #pm v
+  pts_to_serialized (serialize_nlist n s) input #pm v
 returns input' : slice byte
 ensures exists* v' .
   pts_to_serialized s input' #pm v' **
-  trade (pts_to_serialized s input' #pm v') (pts_to_serialized (tot_serialize_nlist n s) input #pm v) **
+  trade (pts_to_serialized s input' #pm v') (pts_to_serialized (serialize_nlist n s) input #pm v) **
   pure (
     Cons? v /\
     v' == List.Tot.hd v
   )
 {
   nlist_cons_as_nondep_then s n input;
-  let res = nondep_then_fst s j (tot_serialize_nlist (n - 1) s) input;
+  let res = nondep_then_fst #_ #(nlist (n - 1) t) s j #(parse_nlist_kind (n - 1) k) #(coerce_eq () (parse_nlist (n - 1) p)) (coerce_eq () (serialize_nlist (n - 1) s <: serializer #(parse_nlist_kind (n - 1) k) (parse_nlist (n - 1) p))) input; // FIXME: WHY WHY WHY are those reveal (hide (...)) NOT reduced?
   Trade.trans (pts_to_serialized s res #pm _) _ _;
   res
 }
@@ -117,28 +117,28 @@ inline_for_extraction
 ```pulse
 fn nlist_tl
   (#t: Type0)
-  (#k: parser_kind)
+  (#k: Ghost.erased parser_kind)
   (#p: parser k t)
   (s: serializer p { k.parser_kind_subkind == Some ParserStrong })
   (j: jumper p)
-  (n: pos)
+  (n: Ghost.erased pos)
   (input: slice byte)
   (#pm: perm)
   (#v: Ghost.erased (nlist n t))
 requires
-  pts_to_serialized (tot_serialize_nlist n s) input #pm v
+  pts_to_serialized (serialize_nlist n s) input #pm v
 returns input' : slice byte
 ensures exists* v' .
-  pts_to_serialized (tot_serialize_nlist (n - 1) s) input' #pm v' **
-  trade (pts_to_serialized (tot_serialize_nlist (n - 1) s) input' #pm v') (pts_to_serialized (tot_serialize_nlist n s) input #pm v) **
+  pts_to_serialized (serialize_nlist (n - 1) s) input' #pm v' **
+  trade (pts_to_serialized (serialize_nlist (n - 1) s) input' #pm v') (pts_to_serialized (serialize_nlist n s) input #pm v) **
   pure (
     Cons? v /\
     v' == List.Tot.tl v
   )
 {
   nlist_cons_as_nondep_then s n input;
-  let res = nondep_then_snd s j (tot_serialize_nlist (n - 1) s) input;
-  Trade.trans (pts_to_serialized (tot_serialize_nlist (n - 1) s) res #pm _) _ _;
+  let res = nondep_then_snd #_ #(nlist (n - 1) t) s j #(parse_nlist_kind (n - 1) k) #(coerce_eq () (parse_nlist (n - 1) p)) (coerce_eq () (serialize_nlist (n - 1) s <: serializer (parse_nlist (n - 1) p))) input; // FIXME: same as above
+  Trade.trans (pts_to_serialized (serialize_nlist (n - 1) s) res #pm _) _ _;
   res
 }
 ```
@@ -147,24 +147,24 @@ inline_for_extraction
 ```pulse
 fn nlist_nth
    (#t: Type0)
-   (#k: parser_kind)
+   (#k: Ghost.erased parser_kind)
    (#p: parser k t)
    (s: serializer p { k.parser_kind_subkind == Some ParserStrong })
    (j: jumper p)
-   (n0: SZ.t)
+   (n0: Ghost.erased nat)
   (input: slice byte)
   (#pm: perm)
-  (#v0: Ghost.erased (nlist (SZ.v n0) t))
-  (i0: SZ.t { SZ.v i0 < SZ.v n0 })
+  (#v0: Ghost.erased (nlist n0 t))
+  (i0: SZ.t { SZ.v i0 < n0 })
 requires
-  pts_to_serialized (tot_serialize_nlist (SZ.v n0) s) input #pm v0
+  pts_to_serialized (serialize_nlist n0 s) input #pm v0
 returns input' : slice byte
 ensures exists* v .
   pts_to_serialized s input' #pm v **
-  trade (pts_to_serialized s input' #pm v) (pts_to_serialized (tot_serialize_nlist (SZ.v n0) s) input #pm v0) **
+  trade (pts_to_serialized s input' #pm v) (pts_to_serialized (serialize_nlist n0 s) input #pm v0) **
   pure (v == List.Tot.index v0 (SZ.v i0))
 {
-  Trade.refl (pts_to_serialized (tot_serialize_nlist (SZ.v n0) s) input #pm v0);
+  Trade.refl (pts_to_serialized (serialize_nlist n0 s) input #pm v0);
   let mut pi = 0sz;
   let mut pres = input;
   while (
@@ -172,26 +172,26 @@ ensures exists* v .
     (SZ.lt i i0)
   ) invariant b . exists* i res (n: nat) (v: nlist n t) . (
     R.pts_to pi i ** R.pts_to pres res **
-    pts_to_serialized (tot_serialize_nlist n s) res #pm v **
-    trade (pts_to_serialized (tot_serialize_nlist n s) res #pm v) (pts_to_serialized (tot_serialize_nlist (SZ.v n0) s) input #pm v0) **
+    pts_to_serialized (serialize_nlist n s) res #pm v **
+    trade (pts_to_serialized (serialize_nlist n s) res #pm v) (pts_to_serialized (serialize_nlist n0 s) input #pm v0) **
     pure (
       SZ.v i <= SZ.v i0 /\
       (b == (SZ.v i < SZ.v i0)) /\
-      n == SZ.v n0 - SZ.v i /\
+      n == n0 - SZ.v i /\
       List.Tot.index v0 (SZ.v i0) == List.Tot.index v (SZ.v i0 - SZ.v i)
   )) {
     let res = !pres;
     let i = !pi;
-    let res2 = nlist_tl s j (SZ.v n0 - SZ.v i) res;
+    let res2 = nlist_tl s j (n0 - SZ.v i) res;
     pi := (SZ.add i 1sz);
     pres := res2;
     Trade.trans
-      (pts_to_serialized (tot_serialize_nlist (SZ.v n0 - SZ.v i - 1) s) res2 #pm _)
+      (pts_to_serialized (serialize_nlist (n0 - SZ.v i - 1) s) res2 #pm _)
       _
       _
   };
   let res = !pres;
-  let res2 = nlist_hd s j (SZ.v n0 - SZ.v i0) res;
+  let res2 = nlist_hd s j (n0 - SZ.v i0) res;
   Trade.trans
     (pts_to_serialized s res2 #pm _) _ _;
   res2
@@ -210,17 +210,18 @@ let synth_nlist_1_recip
 : Tot t
 = List.Tot.hd x
 
-let tot_parse_nlist_1_eq
+let parse_nlist_1_eq
   (#t: Type)
   (#k: parser_kind)
   (p: parser k t)
   (b: bytes)
 : Lemma
-  (parse (tot_parse_nlist 1 p) b == parse (tot_parse_synth p synth_nlist_1) b)
-= tot_parse_nlist_eq 1 p b;
-  tot_parse_synth_eq p synth_nlist_1 b
+  (parse (parse_nlist 1 p) b == parse (parse_synth p synth_nlist_1) b)
+= parse_nlist_eq 1 p b;
+  parse_synth_eq p synth_nlist_1 b
 
 ```pulse
+ghost
 fn pts_to_serialized_nlist_1
   (#t: Type0)
   (#k: parser_kind)
@@ -228,21 +229,21 @@ fn pts_to_serialized_nlist_1
   (s: serializer p { k.parser_kind_subkind == Some ParserStrong })
   (input: slice byte)
   (#pm: perm)
-  (#v: Ghost.erased t)
+  (#v: t)
   requires pts_to_serialized s input #pm v
-  ensures exists* v' . pts_to_serialized (tot_serialize_nlist 1 s) input #pm v' **
-    trade (pts_to_serialized (tot_serialize_nlist 1 s) input #pm v')
+  ensures exists* v' . pts_to_serialized (serialize_nlist 1 s) input #pm v' **
+    trade (pts_to_serialized (serialize_nlist 1 s) input #pm v')
       (pts_to_serialized s input #pm v) **
-    pure ((v' <: list t) == [Ghost.reveal v])
+    pure ((v' <: list t) == [v])
 {
   pts_to_serialized_synth_trade s synth_nlist_1 synth_nlist_1_recip input;
-  Classical.forall_intro (tot_parse_nlist_1_eq p);
+  Classical.forall_intro (parse_nlist_1_eq p);
   pts_to_serialized_ext_trade
-    (tot_serialize_synth p synth_nlist_1 s synth_nlist_1_recip ())
-    (tot_serialize_nlist 1 s)
+    (serialize_synth p synth_nlist_1 s synth_nlist_1_recip ())
+    (serialize_nlist 1 s)
     input;
   Trade.trans
-    (pts_to_serialized (tot_serialize_nlist 1 s) input #pm _)
+    (pts_to_serialized (serialize_nlist 1 s) input #pm _)
     _ _
 }
 ```
