src/lowparse/pulse/LowParse.Pulse.Int.fst
@@ -9,12 +9,12 @@ module SZ = FStar.SizeT
 module S = Pulse.Lib.Slice
 
 inline_for_extraction
-let validate_u8 : validator tot_parse_u8 =
-  validate_total_constant_size tot_parse_u8 1sz
+let validate_u8 : validator parse_u8 =
+  validate_total_constant_size parse_u8 1sz
 
 inline_for_extraction
-let jump_u8 : jumper tot_parse_u8 =
-  jump_constant_size tot_parse_u8 1sz
+let jump_u8 : jumper parse_u8 =
+  jump_constant_size parse_u8 1sz
 
 inline_for_extraction
 noextract
@@ -23,29 +23,29 @@ let be_to_n_1 =  (E.mk_be_to_n EI.uint8 1)
 
 inline_for_extraction
 ```pulse
-fn read_u8' (_: unit) : leaf_reader #FStar.UInt8.t #parse_u8_kind #tot_parse_u8 tot_serialize_u8
+fn read_u8' (_: unit) : leaf_reader #FStar.UInt8.t #parse_u8_kind #parse_u8 serialize_u8
 = (input: S.slice byte)
   (#pm: perm)
   (#v: Ghost.erased FStar.UInt8.t)
 {
-  unfold (pts_to_serialized tot_serialize_u8 input #pm v);
+  unfold (pts_to_serialized serialize_u8 input #pm v);
   serialize_u8_spec_be v;
   let res = be_to_n_1 input 1sz;
-  fold (pts_to_serialized tot_serialize_u8 input #pm v);
+  fold (pts_to_serialized serialize_u8 input #pm v);
   res
 }
 ```
 
 inline_for_extraction
-let read_u8 : reader tot_serialize_u8 = reader_of_leaf_reader (read_u8' ())
+let read_u8 : reader serialize_u8 = reader_of_leaf_reader (read_u8' ())
 
 inline_for_extraction
-let validate_u16 : validator tot_parse_u16 =
-  validate_total_constant_size tot_parse_u16 2sz
+let validate_u16 : validator parse_u16 =
+  validate_total_constant_size parse_u16 2sz
 
 inline_for_extraction
-let jump_u16 : jumper tot_parse_u16 =
-  jump_constant_size tot_parse_u16 2sz
+let jump_u16 : jumper parse_u16 =
+  jump_constant_size parse_u16 2sz
 
 inline_for_extraction
 noextract
@@ -54,29 +54,29 @@ let be_to_n_2 = (E.mk_be_to_n EI.uint16 2)
 
 inline_for_extraction
 ```pulse
-fn read_u16' (_: unit) : leaf_reader #FStar.UInt16.t #parse_u16_kind #tot_parse_u16 tot_serialize_u16
+fn read_u16' (_: unit) : leaf_reader #FStar.UInt16.t #parse_u16_kind #parse_u16 serialize_u16
 = (input: S.slice byte)
   (#pm: perm)
   (#v: Ghost.erased FStar.UInt16.t)
 {
-  unfold (pts_to_serialized tot_serialize_u16 input #pm v);
+  unfold (pts_to_serialized serialize_u16 input #pm v);
   serialize_u16_spec_be v;
   let res = be_to_n_2 input 2sz;
-  fold (pts_to_serialized tot_serialize_u16 input #pm v);
+  fold (pts_to_serialized serialize_u16 input #pm v);
   res
 }
 ```
 
 inline_for_extraction
-let read_u16 : reader tot_serialize_u16 = reader_of_leaf_reader (read_u16' ())
+let read_u16 : reader serialize_u16 = reader_of_leaf_reader (read_u16' ())
 
 inline_for_extraction
-let validate_u32 : validator tot_parse_u32 =
-  validate_total_constant_size tot_parse_u32 4sz
+let validate_u32 : validator parse_u32 =
+  validate_total_constant_size parse_u32 4sz
 
 inline_for_extraction
-let jump_u32 : jumper tot_parse_u32 =
-  jump_constant_size tot_parse_u32 4sz
+let jump_u32 : jumper parse_u32 =
+  jump_constant_size parse_u32 4sz
 
 inline_for_extraction
 noextract
@@ -85,29 +85,29 @@ let be_to_n_4 = (E.mk_be_to_n EI.uint32 4)
 
 inline_for_extraction
 ```pulse
-fn read_u32' (_: unit) : leaf_reader #FStar.UInt32.t #parse_u32_kind #tot_parse_u32 tot_serialize_u32
+fn read_u32' (_: unit) : leaf_reader #FStar.UInt32.t #parse_u32_kind #parse_u32 serialize_u32
 = (input: S.slice byte)
   (#pm: perm)
   (#v: Ghost.erased FStar.UInt32.t)
 {
-  unfold (pts_to_serialized tot_serialize_u32 input #pm v);
+  unfold (pts_to_serialized serialize_u32 input #pm v);
   serialize_u32_spec_be v;
   let res = be_to_n_4 input 4sz;
-  fold (pts_to_serialized tot_serialize_u32 input #pm v);
+  fold (pts_to_serialized serialize_u32 input #pm v);
   res
 }
 ```
 
 inline_for_extraction
-let read_u32 : reader tot_serialize_u32 = reader_of_leaf_reader (read_u32' ())
+let read_u32 : reader serialize_u32 = reader_of_leaf_reader (read_u32' ())
 
 inline_for_extraction
-let validate_u64 : validator tot_parse_u64 =
-  validate_total_constant_size tot_parse_u64 8sz
+let validate_u64 : validator parse_u64 =
+  validate_total_constant_size parse_u64 8sz
 
 inline_for_extraction
-let jump_u64 : jumper tot_parse_u64 =
-  jump_constant_size tot_parse_u64 8sz
+let jump_u64 : jumper parse_u64 =
+  jump_constant_size parse_u64 8sz
 
 inline_for_extraction
 noextract
@@ -116,18 +116,18 @@ let be_to_n_8 = (E.mk_be_to_n EI.uint64 8)
 
 inline_for_extraction
 ```pulse
-fn read_u64' (_: unit) : leaf_reader #FStar.UInt64.t #parse_u64_kind #tot_parse_u64 tot_serialize_u64
+fn read_u64' (_: unit) : leaf_reader #FStar.UInt64.t #parse_u64_kind #parse_u64 serialize_u64
 = (input: S.slice byte)
   (#pm: perm)
   (#v: Ghost.erased FStar.UInt64.t)
 {
-  unfold (pts_to_serialized tot_serialize_u64 input #pm v);
+  unfold (pts_to_serialized serialize_u64 input #pm v);
   serialize_u64_spec_be v;
   let res = be_to_n_8 input 8sz;
-  fold (pts_to_serialized tot_serialize_u64 input #pm v);
+  fold (pts_to_serialized serialize_u64 input #pm v);
   res
 }
 ```
 
 inline_for_extraction
-let read_u64 : reader tot_serialize_u64 = reader_of_leaf_reader (read_u64' ())
+let read_u64 : reader serialize_u64 = reader_of_leaf_reader (read_u64' ())
